<?xml version="1.0" encoding="UTF-8"?>
<rdf:RDF xmlns:rdf="http://www.w3.org/1999/02/22-rdf-syntax-ns#" xmlns:reg="http://purl.org/linked-data/registry#" xmlns:sssom="https://w3id.org/sssom/schema/" xmlns:cpm="http://purl.org/voc/cpm#" xmlns:qudt="https://qudt.org/2.1/schema/qudt#" xmlns:rdfs="http://www.w3.org/2000/01/rdf-schema#" xmlns:void="http://rdfs.org/ns/void#" xmlns:dce="http://purl.org/dc/elements/1.1/" xmlns:dc="http://purl.org/dc/terms/" xmlns:iop="https://w3id.org/iadopt/ont#" xmlns:owl="http://www.w3.org/2002/07/owl#" xmlns:semapv="http://w3id.org/semapv/vocab/" xmlns:grg="http://www.isotc211.org/schemas/grg/" xmlns:ns0="http://www.w3.org/ns/dx/conneg/altr#" xmlns:pav="http://purl.org/pav/" xmlns:skos="http://www.w3.org/2004/02/skos/core#" xmlns:prov="https://www.w3.org/ns/prov#" xmlns:dcat="http://www.w3.org/ns/dcat#" xmlns:ns1="http://www.w3.org/ns/dx/prof/" xmlns:puv="https://w3id.org/env/puv#">
  <rdf:Description rdf:about="http://vocab.nerc.ac.uk/collection/L13/current/LI/">
    <pav:authoredOn>2013-02-05 12:39:17.0</pav:authoredOn>
    <owl:deprecated>false</owl:deprecated>
    <dc:date>2013-02-05 12:39:17.0</dc:date>
    <owl:versionInfo>1</owl:versionInfo>
    <skos:note xml:lang="en">accepted</skos:note>
    <rdf:type rdf:resource="http://www.w3.org/2004/02/skos/core#Concept" />
    <skos:altLabel>littoral</skos:altLabel>
    <pav:hasCurrentVersion rdf:resource="http://vocab.nerc.ac.uk/collection/L13/current/LI/1/" />
    <skos:prefLabel xml:lang="en">littoral</skos:prefLabel>
    <dce:identifier>SDN:L13::LI</dce:identifier>
    <dc:identifier>SDN:L13::LI</dc:identifier>
    <skos:notation>SDN:L13::LI</skos:notation>
    <void:inDataset rdf:resource="http://vocab.nerc.ac.uk/.well-known/void" />
    <pav:version>1</pav:version>
    <skos:definition xml:lang="en">That part of the shore (the fringe of a body of water that has been geologically modified by the action of that body of water past and present) above the low water mark and therefore exposed to the atmosphere at low tide.</skos:definition>
  </rdf:Description>
  <rdf:Description rdf:about="http://vocab.nerc.ac.uk/collection/L13/current/TS/">
    <dc:identifier>SDN:L13::TS</dc:identifier>
    <skos:definition xml:lang="en">The atmospheric layer extending between heights of approximately 80 km to approximately 400 km characterised by rising temperature with height and phenomena associated with ionisation.  Part of the thermosphere is sometimes termed the ionosphere.</skos:definition>
    <skos:prefLabel xml:lang="en">thermosphere</skos:prefLabel>
    <rdf:type rdf:resource="http://www.w3.org/2004/02/skos/core#Concept" />
    <dce:identifier>SDN:L13::TS</dce:identifier>
    <owl:versionInfo>1</owl:versionInfo>
    <void:inDataset rdf:resource="http://vocab.nerc.ac.uk/.well-known/void" />
    <skos:note xml:lang="en">accepted</skos:note>
    <skos:broader rdf:resource="http://vocab.nerc.ac.uk/collection/L19/current/SDNKG16/" />
    <pav:hasCurrentVersion rdf:resource="http://vocab.nerc.ac.uk/collection/L13/current/TS/1/" />
    <dc:date>2006-11-15 08:15:00.0</dc:date>
    <skos:related rdf:resource="http://vocab.nerc.ac.uk/collection/P25/current/ATEMP/" />
    <pav:version>1</pav:version>
    <skos:altLabel>thermosphere</skos:altLabel>
    <owl:deprecated>false</owl:deprecated>
    <pav:authoredOn>2006-11-15 08:15:00.0</pav:authoredOn>
    <skos:notation>SDN:L13::TS</skos:notation>
  </rdf:Description>
  <rdf:Description rdf:about="http://vocab.nerc.ac.uk/collection/L13/current/U2/">
    <skos:broader rdf:resource="http://vocab.nerc.ac.uk/collection/L19/current/SDNKG16/" />
    <pav:authoredOn>2006-11-15 08:15:00.0</pav:authoredOn>
    <skos:prefLabel xml:lang="en">epipelagic water column</skos:prefLabel>
    <void:inDataset rdf:resource="http://vocab.nerc.ac.uk/.well-known/void" />
    <skos:related rdf:resource="http://vocab.nerc.ac.uk/collection/P25/current/PHYTABUND/" />
    <skos:related rdf:resource="http://vocab.nerc.ac.uk/collection/P25/current/NO2/" />
    <pav:version>1</pav:version>
    <skos:related rdf:resource="http://vocab.nerc.ac.uk/collection/P25/current/SALIN/" />
    <skos:definition xml:lang="en">The water column zone in which for clear water there is adequate light for photosynthesis. Typically from  the surface down to a depth of approximately 200 metres.</skos:definition>
    <skos:altLabel>epipelagic</skos:altLabel>
    <skos:related rdf:resource="http://vocab.nerc.ac.uk/collection/P25/current/PHAEO/" />
    <dce:identifier>SDN:L13::U2</dce:identifier>
    <skos:related rdf:resource="http://vocab.nerc.ac.uk/collection/P25/current/CHLA/" />
    <dc:identifier>SDN:L13::U2</dc:identifier>
    <owl:versionInfo>1</owl:versionInfo>
    <skos:related rdf:resource="http://vocab.nerc.ac.uk/collection/P25/current/NO3NO2/" />
    <skos:related rdf:resource="http://vocab.nerc.ac.uk/collection/P25/current/SLCA/" />
    <skos:note xml:lang="en">accepted</skos:note>
    <skos:related rdf:resource="http://vocab.nerc.ac.uk/collection/P25/current/WTEMP/" />
    <owl:deprecated>false</owl:deprecated>
    <skos:related rdf:resource="http://vocab.nerc.ac.uk/collection/P25/current/PO4/" />
    <skos:notation>SDN:L13::U2</skos:notation>
    <skos:related rdf:resource="http://vocab.nerc.ac.uk/collection/P25/current/NO3/" />
    <dc:date>2006-11-15 08:15:00.0</dc:date>
    <rdf:type rdf:resource="http://www.w3.org/2004/02/skos/core#Concept" />
    <pav:hasCurrentVersion rdf:resource="http://vocab.nerc.ac.uk/collection/L13/current/U2/1/" />
  </rdf:Description>
  <rdf:Description rdf:about="http://vocab.nerc.ac.uk/collection/L13/current/AY/">
    <owl:deprecated>false</owl:deprecated>
    <rdf:type rdf:resource="http://www.w3.org/2004/02/skos/core#Concept" />
    <dce:identifier>SDN:L13::AY</dce:identifier>
    <skos:definition xml:lang="en">The zone of the seabed comprising the ocean floor with a bathymetric depth greater than  approximately 2700 metres where the bathyal fauna are replaced by more primitive abyssal fauna.</skos:definition>
    <pav:authoredOn>2013-02-05 12:39:17.0</pav:authoredOn>
    <skos:note xml:lang="en">accepted</skos:note>
    <owl:versionInfo>1</owl:versionInfo>
    <dc:identifier>SDN:L13::AY</dc:identifier>
    <skos:notation>SDN:L13::AY</skos:notation>
    <skos:altLabel>abyssobenthic</skos:altLabel>
    <pav:version>1</pav:version>
    <pav:hasCurrentVersion rdf:resource="http://vocab.nerc.ac.uk/collection/L13/current/AY/1/" />
    <void:inDataset rdf:resource="http://vocab.nerc.ac.uk/.well-known/void" />
    <dc:date>2013-02-05 12:39:17.0</dc:date>
    <skos:prefLabel xml:lang="en">abyssobenthic</skos:prefLabel>
  </rdf:Description>
  <rdf:Description rdf:about="http://vocab.nerc.ac.uk/collection/L13/current/U1/">
    <skos:related rdf:resource="http://vocab.nerc.ac.uk/collection/P25/current/SALIN/" />
    <skos:note xml:lang="en">accepted</skos:note>
    <skos:related rdf:resource="http://vocab.nerc.ac.uk/collection/P25/current/NO2/" />
    <skos:related rdf:resource="http://vocab.nerc.ac.uk/collection/P25/current/PHAEO/" />
    <dce:identifier>SDN:L13::U1</dce:identifier>
    <skos:notation>SDN:L13::U1</skos:notation>
    <dc:date>2006-11-15 08:15:00.0</dc:date>
    <skos:related rdf:resource="http://vocab.nerc.ac.uk/collection/P25/current/NO3/" />
    <skos:related rdf:resource="http://vocab.nerc.ac.uk/collection/P25/current/SLCA/" />
    <skos:related rdf:resource="http://vocab.nerc.ac.uk/collection/P25/current/WTEMP/" />
    <skos:related rdf:resource="http://vocab.nerc.ac.uk/collection/P25/current/PO4/" />
    <owl:versionInfo>1</owl:versionInfo>
    <skos:related rdf:resource="http://vocab.nerc.ac.uk/collection/P25/current/NO3NO2/" />
    <pav:hasCurrentVersion rdf:resource="http://vocab.nerc.ac.uk/collection/L13/current/U1/1/" />
    <dc:identifier>SDN:L13::U1</dc:identifier>
    <rdf:type rdf:resource="http://www.w3.org/2004/02/skos/core#Concept" />
    <pav:authoredOn>2006-11-15 08:15:00.0</pav:authoredOn>
    <skos:definition xml:lang="en">The strongly illuminated upper half of the epipelagic zone. Typically from the surface down to a depth of approximately 100 metres.</skos:definition>
    <owl:deprecated>false</owl:deprecated>
    <skos:altLabel>upper_epipelagic</skos:altLabel>
    <skos:related rdf:resource="http://vocab.nerc.ac.uk/collection/P25/current/PHYTABUND/" />
    <skos:related rdf:resource="http://vocab.nerc.ac.uk/collection/P25/current/CHLA/" />
    <skos:prefLabel xml:lang="en">upper epipelagic water column</skos:prefLabel>
    <void:inDataset rdf:resource="http://vocab.nerc.ac.uk/.well-known/void" />
    <pav:version>1</pav:version>
    <skos:broader rdf:resource="http://vocab.nerc.ac.uk/collection/L19/current/SDNKG16/" />
  </rdf:Description>
  <rdf:Description rdf:about="http://vocab.nerc.ac.uk/collection/L13/current/TP/">
    <skos:note xml:lang="en">accepted</skos:note>
    <dce:identifier>SDN:L13::TP</dce:identifier>
    <skos:notation>SDN:L13::TP</skos:notation>
    <dc:date>2006-11-15 08:15:00.0</dc:date>
    <skos:definition xml:lang="en">The boundary between the troposphere and stratosphere, characterized by change in temperature gradient with height from decreasing below to increasing above. May extend over a few km in height. Typically lies somewhere between 10 and 15 km.</skos:definition>
    <owl:versionInfo>1</owl:versionInfo>
    <pav:hasCurrentVersion rdf:resource="http://vocab.nerc.ac.uk/collection/L13/current/TP/1/" />
    <dc:identifier>SDN:L13::TP</dc:identifier>
    <skos:altLabel>tropopause</skos:altLabel>
    <rdf:type rdf:resource="http://www.w3.org/2004/02/skos/core#Concept" />
    <pav:authoredOn>2006-11-15 08:15:00.0</pav:authoredOn>
    <owl:deprecated>false</owl:deprecated>
    <skos:prefLabel xml:lang="en">tropopause</skos:prefLabel>
    <skos:related rdf:resource="http://vocab.nerc.ac.uk/collection/P25/current/ATEMP/" />
    <void:inDataset rdf:resource="http://vocab.nerc.ac.uk/.well-known/void" />
    <pav:version>1</pav:version>
    <skos:broader rdf:resource="http://vocab.nerc.ac.uk/collection/L19/current/SDNKG16/" />
  </rdf:Description>
  <rdf:Description rdf:about="http://vocab.nerc.ac.uk/collection/L13/current/DC/">
    <pav:hasCurrentVersion rdf:resource="http://vocab.nerc.ac.uk/collection/L13/current/DC/1/" />
    <skos:altLabel>offshore_circalittoral</skos:altLabel>
    <pav:authoredOn>2013-02-05 12:39:17.0</pav:authoredOn>
    <skos:notation>SDN:L13::DC</skos:notation>
    <skos:note xml:lang="en">accepted</skos:note>
    <dc:identifier>SDN:L13::DC</dc:identifier>
    <void:inDataset rdf:resource="http://vocab.nerc.ac.uk/.well-known/void" />
    <skos:definition xml:lang="en">The zone of the seabed between the depth to which storms and waves still influence the seabed (wave-base) and the marked break of slope that characterises the offshore limit of the shelf (shelf-break).</skos:definition>
    <owl:deprecated>false</owl:deprecated>
    <owl:versionInfo>1</owl:versionInfo>
    <pav:version>1</pav:version>
    <rdf:type rdf:resource="http://www.w3.org/2004/02/skos/core#Concept" />
    <dc:date>2013-02-05 12:39:17.0</dc:date>
    <skos:prefLabel xml:lang="en">deep circalittoral</skos:prefLabel>
    <dce:identifier>SDN:L13::DC</dce:identifier>
  </rdf:Description>
  <rdf:Description rdf:about="http://vocab.nerc.ac.uk/collection/L13/current/BB/">
    <skos:notation>SDN:L13::BB</skos:notation>
    <skos:prefLabel xml:lang="en">bathybenthic</skos:prefLabel>
    <skos:note xml:lang="en">accepted</skos:note>
    <void:inDataset rdf:resource="http://vocab.nerc.ac.uk/.well-known/void" />
    <owl:deprecated>false</owl:deprecated>
    <skos:definition xml:lang="en">The zone of the seabed between the permanent thermocline in the overlying water body and the limit of colonisation by bathyal fauna. It incorporates the lower part of the slope and the ocean floor to around 2700 metres bathymetric depth. It includes several faunal discontinuities.</skos:definition>
    <skos:altLabel>bathybenthic</skos:altLabel>
    <pav:hasVersion rdf:resource="http://vocab.nerc.ac.uk/collection/L13/current/BB/1/" />
    <pav:hasCurrentVersion rdf:resource="http://vocab.nerc.ac.uk/collection/L13/current/BB/2/" />
    <pav:version>2</pav:version>
    <dc:date>2020-05-20 21:09:54.0</dc:date>
    <pav:authoredOn>2020-05-20 21:09:54.0</pav:authoredOn>
    <owl:versionInfo>2</owl:versionInfo>
    <dce:identifier>SDN:L13::BB</dce:identifier>
    <dc:identifier>SDN:L13::BB</dc:identifier>
    <rdf:type rdf:resource="http://www.w3.org/2004/02/skos/core#Concept" />
  </rdf:Description>
  <rdf:Description rdf:about="http://vocab.nerc.ac.uk/collection/L13/current/TH/">
    <pav:version>1</pav:version>
    <skos:altLabel>troposphere</skos:altLabel>
    <owl:versionInfo>1</owl:versionInfo>
    <skos:notation>SDN:L13::TH</skos:notation>
    <skos:definition xml:lang="en">The  lowest broad layer of the atmosphere characterised by decreasing avearage temperature with height.  Typically from the surface to between 10 and 15 km.</skos:definition>
    <owl:deprecated>false</owl:deprecated>
    <dc:date>2006-11-15 08:15:00.0</dc:date>
    <void:inDataset rdf:resource="http://vocab.nerc.ac.uk/.well-known/void" />
    <pav:authoredOn>2006-11-15 08:15:00.0</pav:authoredOn>
    <skos:prefLabel xml:lang="en">troposphere</skos:prefLabel>
    <skos:broader rdf:resource="http://vocab.nerc.ac.uk/collection/L19/current/SDNKG16/" />
    <dce:identifier>SDN:L13::TH</dce:identifier>
    <pav:hasCurrentVersion rdf:resource="http://vocab.nerc.ac.uk/collection/L13/current/TH/1/" />
    <dc:identifier>SDN:L13::TH</dc:identifier>
    <skos:related rdf:resource="http://vocab.nerc.ac.uk/collection/P25/current/ATEMP/" />
    <rdf:type rdf:resource="http://www.w3.org/2004/02/skos/core#Concept" />
    <skos:note xml:lang="en">accepted</skos:note>
  </rdf:Description>
  <rdf:Description rdf:about="http://vocab.nerc.ac.uk/collection/L13/current/CO/">
    <owl:deprecated>false</owl:deprecated>
    <skos:note xml:lang="en">accepted</skos:note>
    <dce:identifier>SDN:L13::CO</dce:identifier>
    <rdf:type rdf:resource="http://www.w3.org/2004/02/skos/core#Concept" />
    <skos:broader rdf:resource="http://vocab.nerc.ac.uk/collection/L19/current/SDNKG16/" />
    <skos:definition xml:lang="en">The central zone of the earth largely composed of solid or molten metal alloys, typically from the centre of the Earth to approximately 2900 km below the surface..</skos:definition>
    <skos:altLabel>core</skos:altLabel>
    <void:inDataset rdf:resource="http://vocab.nerc.ac.uk/.well-known/void" />
    <pav:authoredOn>2006-11-15 08:15:00.0</pav:authoredOn>
    <pav:hasCurrentVersion rdf:resource="http://vocab.nerc.ac.uk/collection/L13/current/CO/1/" />
    <skos:notation>SDN:L13::CO</skos:notation>
    <dc:identifier>SDN:L13::CO</dc:identifier>
    <dc:date>2006-11-15 08:15:00.0</dc:date>
    <pav:version>1</pav:version>
    <owl:versionInfo>1</owl:versionInfo>
    <skos:prefLabel xml:lang="en">core</skos:prefLabel>
  </rdf:Description>
  <rdf:Description rdf:about="http://vocab.nerc.ac.uk/collection/L13/current/CL/">
    <pav:authoredOn>2013-02-05 12:39:17.0</pav:authoredOn>
    <skos:prefLabel xml:lang="en">circalittoral</skos:prefLabel>
    <skos:altLabel>circalittoral</skos:altLabel>
    <rdf:type rdf:resource="http://www.w3.org/2004/02/skos/core#Concept" />
    <owl:versionInfo>1</owl:versionInfo>
    <pav:hasCurrentVersion rdf:resource="http://vocab.nerc.ac.uk/collection/L13/current/CL/1/" />
    <skos:note xml:lang="en">accepted</skos:note>
    <pav:version>1</pav:version>
    <skos:notation>SDN:L13::CL</skos:notation>
    <owl:deprecated>false</owl:deprecated>
    <skos:definition xml:lang="en">The zone of the seabed dominated by animals. On open coastline this is from bottom of the infralittoral zone to the depth to which storms and waves still influence the seabed (wave-base).</skos:definition>
    <void:inDataset rdf:resource="http://vocab.nerc.ac.uk/.well-known/void" />
    <dc:date>2013-02-05 12:39:17.0</dc:date>
    <dc:identifier>SDN:L13::CL</dc:identifier>
    <dce:identifier>SDN:L13::CL</dce:identifier>
  </rdf:Description>
  <rdf:Description rdf:about="http://vocab.nerc.ac.uk/collection/L13/current/NB/">
    <pav:authoredOn>2006-11-15 08:15:00.0</pav:authoredOn>
    <skos:related rdf:resource="http://vocab.nerc.ac.uk/collection/P25/current/PO4/" />
    <skos:related rdf:resource="http://vocab.nerc.ac.uk/collection/P25/current/SALIN/" />
    <skos:notation>SDN:L13::NB</skos:notation>
    <skos:altLabel>benthic_boundary</skos:altLabel>
    <dc:identifier>SDN:L13::NB</dc:identifier>
    <skos:related rdf:resource="http://vocab.nerc.ac.uk/collection/P25/current/NO3NO2/" />
    <skos:related rdf:resource="http://vocab.nerc.ac.uk/collection/P25/current/NO2/" />
    <pav:hasCurrentVersion rdf:resource="http://vocab.nerc.ac.uk/collection/L13/current/NB/1/" />
    <dce:identifier>SDN:L13::NB</dce:identifier>
    <pav:version>1</pav:version>
    <owl:deprecated>false</owl:deprecated>
    <void:inDataset rdf:resource="http://vocab.nerc.ac.uk/.well-known/void" />
    <dc:date>2006-11-15 08:15:00.0</dc:date>
    <skos:note xml:lang="en">accepted</skos:note>
    <skos:related rdf:resource="http://vocab.nerc.ac.uk/collection/P25/current/SLCA/" />
    <skos:broader rdf:resource="http://vocab.nerc.ac.uk/collection/L19/current/SDNKG16/" />
    <skos:prefLabel xml:lang="en">benthic boundary layer</skos:prefLabel>
    <skos:related rdf:resource="http://vocab.nerc.ac.uk/collection/P25/current/WTEMP/" />
    <owl:versionInfo>1</owl:versionInfo>
    <skos:definition xml:lang="en">The water column that is significantly influenced by the seabed, which is broader in deep ocean than in shelf seas.  Guideline approximation is bottom 10m of oceans and bottom 5% of shelf (&lt;200m) seas.</skos:definition>
    <rdf:type rdf:resource="http://www.w3.org/2004/02/skos/core#Concept" />
    <skos:related rdf:resource="http://vocab.nerc.ac.uk/collection/P25/current/NO3/" />
  </rdf:Description>
  <rdf:Description rdf:about="http://vocab.nerc.ac.uk/collection/L13/current/MS/">
    <dc:date>2006-11-15 08:15:00.0</dc:date>
    <skos:notation>SDN:L13::MS</skos:notation>
    <owl:versionInfo>1</owl:versionInfo>
    <pav:hasCurrentVersion rdf:resource="http://vocab.nerc.ac.uk/collection/L13/current/MS/1/" />
    <skos:related rdf:resource="http://vocab.nerc.ac.uk/collection/P25/current/ATEMP/" />
    <dc:identifier>SDN:L13::MS</dc:identifier>
    <rdf:type rdf:resource="http://www.w3.org/2004/02/skos/core#Concept" />
    <void:inDataset rdf:resource="http://vocab.nerc.ac.uk/.well-known/void" />
    <pav:authoredOn>2006-11-15 08:15:00.0</pav:authoredOn>
    <skos:prefLabel xml:lang="en">mesosphere</skos:prefLabel>
    <skos:definition xml:lang="en">The layer of atmosphere overlying the stratospause characterised by decreasing temperature with height, typically from about 50 to about 80 km</skos:definition>
    <pav:version>1</pav:version>
    <skos:broader rdf:resource="http://vocab.nerc.ac.uk/collection/L19/current/SDNKG16/" />
    <dce:identifier>SDN:L13::MS</dce:identifier>
    <skos:note xml:lang="en">accepted</skos:note>
    <skos:altLabel>mesosphere</skos:altLabel>
    <owl:deprecated>false</owl:deprecated>
  </rdf:Description>
  <rdf:Description rdf:about="http://vocab.nerc.ac.uk/collection/L13/current/AT/">
    <skos:notation>SDN:L13::AT</skos:notation>
    <skos:note xml:lang="en">accepted</skos:note>
    <void:inDataset rdf:resource="http://vocab.nerc.ac.uk/.well-known/void" />
    <skos:inScheme rdf:resource="http://vocab.nerc.ac.uk/scheme/NETOC_VCOV/current/" />
    <skos:definition xml:lang="en">The envelope of gases surrounding the Earth.</skos:definition>
    <pav:hasCurrentVersion rdf:resource="http://vocab.nerc.ac.uk/collection/L13/current/AT/1/" />
    <skos:related rdf:resource="http://vocab.nerc.ac.uk/collection/P25/current/ATEMP/" />
    <pav:version>1</pav:version>
    <skos:broader rdf:resource="http://vocab.nerc.ac.uk/collection/L19/current/SDNKG16/" />
    <skos:altLabel>atmosphere</skos:altLabel>
    <skos:altLabel xml:lang="en">atmosphere</skos:altLabel>
    <rdf:type rdf:resource="http://www.w3.org/2004/02/skos/core#Concept" />
    <dc:identifier>SDN:L13::AT</dc:identifier>
    <dce:identifier>SDN:L13::AT</dce:identifier>
    <skos:inScheme rdf:resource="http://vocab.nerc.ac.uk/scheme/NETMAR_OCEAN/current/" />
    <owl:deprecated>false</owl:deprecated>
    <skos:prefLabel xml:lang="en">atmosphere</skos:prefLabel>
    <pav:authoredOn>2006-11-15 08:15:00.0</pav:authoredOn>
    <dc:date>2006-11-15 08:15:00.0</dc:date>
    <owl:versionInfo>1</owl:versionInfo>
  </rdf:Description>
  <rdf:Description rdf:about="http://vocab.nerc.ac.uk/collection/L13/current/CR/">
    <void:inDataset rdf:resource="http://vocab.nerc.ac.uk/.well-known/void" />
    <rdf:type rdf:resource="http://www.w3.org/2004/02/skos/core#Concept" />
    <skos:broader rdf:resource="http://vocab.nerc.ac.uk/collection/L19/current/SDNKG16/" />
    <owl:deprecated>false</owl:deprecated>
    <dc:date>2006-11-15 08:15:00.0</dc:date>
    <dc:identifier>SDN:L13::CR</dc:identifier>
    <skos:definition xml:lang="en">The layer of lithified rock between the unconsolidated sediment and the Moho seismic discontinuity. Typically 5-10 km thick beneath oceans and 60-70 km thick beneath continents.</skos:definition>
    <pav:hasCurrentVersion rdf:resource="http://vocab.nerc.ac.uk/collection/L13/current/CR/1/" />
    <skos:altLabel>crust</skos:altLabel>
    <pav:version>1</pav:version>
    <skos:note xml:lang="en">accepted</skos:note>
    <pav:authoredOn>2006-11-15 08:15:00.0</pav:authoredOn>
    <dce:identifier>SDN:L13::CR</dce:identifier>
    <skos:prefLabel xml:lang="en">crust</skos:prefLabel>
    <skos:notation>SDN:L13::CR</skos:notation>
    <owl:versionInfo>1</owl:versionInfo>
  </rdf:Description>
  <rdf:Description rdf:about="http://vocab.nerc.ac.uk/collection/L13/current/MW/">
    <pav:authoredOn>2006-11-15 08:15:00.0</pav:authoredOn>
    <rdf:type rdf:resource="http://www.w3.org/2004/02/skos/core#Concept" />
    <skos:related rdf:resource="http://vocab.nerc.ac.uk/collection/P25/current/PO4/" />
    <skos:altLabel>mesopelagic</skos:altLabel>
    <skos:related rdf:resource="http://vocab.nerc.ac.uk/collection/P25/current/SLCA/" />
    <skos:definition xml:lang="en">The water column zone penetrated by light, but in insufficient quantities for photosynthesis. Typically between depths of approximately 200 metres and 1000 metres.</skos:definition>
    <skos:notation>SDN:L13::MW</skos:notation>
    <skos:related rdf:resource="http://vocab.nerc.ac.uk/collection/P25/current/SALIN/" />
    <void:inDataset rdf:resource="http://vocab.nerc.ac.uk/.well-known/void" />
    <skos:related rdf:resource="http://vocab.nerc.ac.uk/collection/P25/current/NO3/" />
    <dc:identifier>SDN:L13::MW</dc:identifier>
    <owl:versionInfo>1</owl:versionInfo>
    <dce:identifier>SDN:L13::MW</dce:identifier>
    <owl:deprecated>false</owl:deprecated>
    <pav:hasCurrentVersion rdf:resource="http://vocab.nerc.ac.uk/collection/L13/current/MW/1/" />
    <skos:related rdf:resource="http://vocab.nerc.ac.uk/collection/P25/current/NO2/" />
    <pav:version>1</pav:version>
    <skos:related rdf:resource="http://vocab.nerc.ac.uk/collection/P25/current/WTEMP/" />
    <skos:prefLabel xml:lang="en">mesopelagic water column</skos:prefLabel>
    <skos:note xml:lang="en">accepted</skos:note>
    <dc:date>2006-11-15 08:15:00.0</dc:date>
    <skos:broader rdf:resource="http://vocab.nerc.ac.uk/collection/L19/current/SDNKG16/" />
    <skos:related rdf:resource="http://vocab.nerc.ac.uk/collection/P25/current/NO3NO2/" />
  </rdf:Description>
  <rdf:Description rdf:about="http://vocab.nerc.ac.uk/collection/L13/current/ES/">
    <void:inDataset rdf:resource="http://vocab.nerc.ac.uk/.well-known/void" />
    <rdf:type rdf:resource="http://www.w3.org/2004/02/skos/core#Concept" />
    <skos:definition xml:lang="en">The outermost layer of the atmosphere from which atoms can escape into outer space. Lies above the thermosphere from about 400 km in altitude.</skos:definition>
    <skos:note xml:lang="en">accepted</skos:note>
    <dce:identifier>SDN:L13::ES</dce:identifier>
    <owl:deprecated>false</owl:deprecated>
    <skos:broader rdf:resource="http://vocab.nerc.ac.uk/collection/L19/current/SDNKG16/" />
    <skos:notation>SDN:L13::ES</skos:notation>
    <pav:hasCurrentVersion rdf:resource="http://vocab.nerc.ac.uk/collection/L13/current/ES/1/" />
    <pav:version>1</pav:version>
    <dc:identifier>SDN:L13::ES</dc:identifier>
    <pav:authoredOn>2006-11-15 08:15:00.0</pav:authoredOn>
    <skos:altLabel>exosphere</skos:altLabel>
    <owl:versionInfo>1</owl:versionInfo>
    <skos:prefLabel xml:lang="en">exosphere</skos:prefLabel>
    <dc:date>2006-11-15 08:15:00.0</dc:date>
  </rdf:Description>
  <rdf:Description rdf:about="http://vocab.nerc.ac.uk/collection/L13/current/AP/">
    <skos:altLabel>abyssopelagic</skos:altLabel>
    <owl:deprecated>false</owl:deprecated>
    <void:inDataset rdf:resource="http://vocab.nerc.ac.uk/.well-known/void" />
    <pav:authoredOn>2006-11-15 08:15:00.0</pav:authoredOn>
    <skos:related rdf:resource="http://vocab.nerc.ac.uk/collection/P25/current/NO3/" />
    <dc:date>2006-11-15 08:15:00.0</dc:date>
    <skos:related rdf:resource="http://vocab.nerc.ac.uk/collection/P25/current/WTEMP/" />
    <dce:identifier>SDN:L13::AP</dce:identifier>
    <skos:broader rdf:resource="http://vocab.nerc.ac.uk/collection/L19/current/SDNKG16/" />
    <pav:hasCurrentVersion rdf:resource="http://vocab.nerc.ac.uk/collection/L13/current/AP/1/" />
    <pav:version>1</pav:version>
    <skos:related rdf:resource="http://vocab.nerc.ac.uk/collection/P25/current/SLCA/" />
    <skos:related rdf:resource="http://vocab.nerc.ac.uk/collection/P25/current/SALIN/" />
    <skos:related rdf:resource="http://vocab.nerc.ac.uk/collection/P25/current/NO3NO2/" />
    <owl:versionInfo>1</owl:versionInfo>
    <rdf:type rdf:resource="http://www.w3.org/2004/02/skos/core#Concept" />
    <skos:definition xml:lang="en">The water column zone of total darkness extending down to the abyssal sea floor. Typically between depths of approximately 4000 metres and 6000 metres.</skos:definition>
    <dc:identifier>SDN:L13::AP</dc:identifier>
    <skos:note xml:lang="en">accepted</skos:note>
    <skos:notation>SDN:L13::AP</skos:notation>
    <skos:related rdf:resource="http://vocab.nerc.ac.uk/collection/P25/current/NO2/" />
    <skos:related rdf:resource="http://vocab.nerc.ac.uk/collection/P25/current/PO4/" />
    <skos:prefLabel xml:lang="en">abyssopelagic water column</skos:prefLabel>
  </rdf:Description>
  <rdf:Description rdf:about="http://vocab.nerc.ac.uk/collection/L13/current/MP/">
    <pav:authoredOn>2006-11-15 08:15:00.0</pav:authoredOn>
    <dce:identifier>SDN:L13::MP</dce:identifier>
    <skos:altLabel>mesopause</skos:altLabel>
    <skos:related rdf:resource="http://vocab.nerc.ac.uk/collection/P25/current/ATEMP/" />
    <skos:note xml:lang="en">accepted</skos:note>
    <skos:prefLabel xml:lang="en">mesopause</skos:prefLabel>
    <owl:deprecated>false</owl:deprecated>
    <void:inDataset rdf:resource="http://vocab.nerc.ac.uk/.well-known/void" />
    <dc:date>2006-11-15 08:15:00.0</dc:date>
    <skos:broader rdf:resource="http://vocab.nerc.ac.uk/collection/L19/current/SDNKG16/" />
    <pav:version>1</pav:version>
    <dc:identifier>SDN:L13::MP</dc:identifier>
    <pav:hasCurrentVersion rdf:resource="http://vocab.nerc.ac.uk/collection/L13/current/MP/1/" />
    <rdf:type rdf:resource="http://www.w3.org/2004/02/skos/core#Concept" />
    <skos:notation>SDN:L13::MP</skos:notation>
    <skos:definition xml:lang="en">The boundary between the mesosphere and the thermosphere characterised by a temperature minimum.  Typically lies somewhere between 80 and 90 km.</skos:definition>
    <owl:versionInfo>1</owl:versionInfo>
  </rdf:Description>
  <rdf:Description rdf:about="http://vocab.nerc.ac.uk/collection/L13/current/SP/">
    <owl:deprecated>false</owl:deprecated>
    <pav:version>1</pav:version>
    <dc:identifier>SDN:L13::SP</dc:identifier>
    <pav:authoredOn>2006-11-15 08:15:00.0</pav:authoredOn>
    <owl:versionInfo>1</owl:versionInfo>
    <skos:notation>SDN:L13::SP</skos:notation>
    <skos:note xml:lang="en">accepted</skos:note>
    <pav:hasCurrentVersion rdf:resource="http://vocab.nerc.ac.uk/collection/L13/current/SP/1/" />
    <skos:related rdf:resource="http://vocab.nerc.ac.uk/collection/P25/current/ATEMP/" />
    <skos:definition xml:lang="en">The boundary between the stratosphere and the mesosphere characterised by a temperature maximum. Typically at about 50 km.</skos:definition>
    <rdf:type rdf:resource="http://www.w3.org/2004/02/skos/core#Concept" />
    <dc:date>2006-11-15 08:15:00.0</dc:date>
    <skos:prefLabel xml:lang="en">stratopause</skos:prefLabel>
    <skos:altLabel>stratopause</skos:altLabel>
    <void:inDataset rdf:resource="http://vocab.nerc.ac.uk/.well-known/void" />
    <dce:identifier>SDN:L13::SP</dce:identifier>
    <skos:broader rdf:resource="http://vocab.nerc.ac.uk/collection/L19/current/SDNKG16/" />
  </rdf:Description>
  <rdf:Description rdf:about="http://vocab.nerc.ac.uk/collection/L13/current/SS/">
    <skos:broader rdf:resource="http://vocab.nerc.ac.uk/collection/L19/current/SDNKG16/" />
    <skos:notation>SDN:L13::SS</skos:notation>
    <dce:identifier>SDN:L13::SS</dce:identifier>
    <pav:version>1</pav:version>
    <dc:identifier>SDN:L13::SS</dc:identifier>
    <rdf:type rdf:resource="http://www.w3.org/2004/02/skos/core#Concept" />
    <owl:versionInfo>1</owl:versionInfo>
    <skos:altLabel>stratosphere</skos:altLabel>
    <skos:prefLabel xml:lang="en">stratosphere</skos:prefLabel>
    <void:inDataset rdf:resource="http://vocab.nerc.ac.uk/.well-known/void" />
    <skos:definition xml:lang="en">The layer of the atmosphere from the tropopause to a height of approximately 50 km, characterised by increasing temperature with height.</skos:definition>
    <owl:deprecated>false</owl:deprecated>
    <skos:note xml:lang="en">accepted</skos:note>
    <pav:hasCurrentVersion rdf:resource="http://vocab.nerc.ac.uk/collection/L13/current/SS/1/" />
    <dc:date>2006-11-15 08:15:00.0</dc:date>
    <skos:related rdf:resource="http://vocab.nerc.ac.uk/collection/P25/current/ATEMP/" />
    <pav:authoredOn>2006-11-15 08:15:00.0</pav:authoredOn>
  </rdf:Description>
  <rdf:Description rdf:about="http://vocab.nerc.ac.uk/collection/L13/current/IL/">
    <dc:identifier>SDN:L13::IL</dc:identifier>
    <rdf:type rdf:resource="http://www.w3.org/2004/02/skos/core#Concept" />
    <owl:deprecated>false</owl:deprecated>
    <void:inDataset rdf:resource="http://vocab.nerc.ac.uk/.well-known/void" />
    <dc:date>2013-02-05 12:39:17.0</dc:date>
    <pav:hasCurrentVersion rdf:resource="http://vocab.nerc.ac.uk/collection/L13/current/IL/1/" />
    <skos:prefLabel xml:lang="en">infralittoral</skos:prefLabel>
    <pav:version>1</pav:version>
    <dce:identifier>SDN:L13::IL</dce:identifier>
    <skos:altLabel>infralittoral</skos:altLabel>
    <skos:note xml:lang="en">accepted</skos:note>
    <skos:definition xml:lang="en">The zone of the seabed dominated by macroalgae below the low water mark. It extends to a depth where 1% of the surface illumination reaches the seabed, which varies according to turbidity.</skos:definition>
    <pav:authoredOn>2013-02-05 12:39:17.0</pav:authoredOn>
    <owl:versionInfo>1</owl:versionInfo>
    <skos:notation>SDN:L13::IL</skos:notation>
  </rdf:Description>
  <rdf:Description rdf:about="http://vocab.nerc.ac.uk/collection/L13/current/US/">
    <skos:note xml:lang="en">accepted</skos:note>
    <skos:altLabel>upper_slope</skos:altLabel>
    <skos:definition xml:lang="en">The zone of steeply-sloping seabed between the shelf-break and the permanent thermocline in the overlying water body.</skos:definition>
    <rdf:type rdf:resource="http://www.w3.org/2004/02/skos/core#Concept" />
    <void:inDataset rdf:resource="http://vocab.nerc.ac.uk/.well-known/void" />
    <skos:prefLabel xml:lang="en">upper slope</skos:prefLabel>
    <owl:versionInfo>1</owl:versionInfo>
    <owl:deprecated>false</owl:deprecated>
    <dc:identifier>SDN:L13::US</dc:identifier>
    <skos:notation>SDN:L13::US</skos:notation>
    <pav:hasCurrentVersion rdf:resource="http://vocab.nerc.ac.uk/collection/L13/current/US/1/" />
    <pav:version>1</pav:version>
    <dc:date>2013-02-05 12:39:17.0</dc:date>
    <pav:authoredOn>2013-02-05 12:39:17.0</pav:authoredOn>
    <dce:identifier>SDN:L13::US</dce:identifier>
  </rdf:Description>
  <rdf:Description rdf:about="http://vocab.nerc.ac.uk/collection/L13/current/WS/">
    <skos:definition xml:lang="en">The zone a few microns thick at the extreme surface of the water column that is sampled by radiometers.</skos:definition>
    <pav:hasCurrentVersion rdf:resource="http://vocab.nerc.ac.uk/collection/L13/current/WS/1/" />
    <skos:broader rdf:resource="http://vocab.nerc.ac.uk/collection/L19/current/SDNKG16/" />
    <skos:inScheme rdf:resource="http://vocab.nerc.ac.uk/scheme/NETMAR_OCEAN/current/" />
    <pav:version>1</pav:version>
    <skos:related rdf:resource="http://vocab.nerc.ac.uk/collection/P25/current/WTEMP/" />
    <pav:authoredOn>2006-11-15 08:15:00.0</pav:authoredOn>
    <skos:inScheme rdf:resource="http://vocab.nerc.ac.uk/scheme/NETOC_VCOV/current/" />
    <owl:versionInfo>1</owl:versionInfo>
    <owl:deprecated>false</owl:deprecated>
    <dce:identifier>SDN:L13::WS</dce:identifier>
    <skos:notation>SDN:L13::WS</skos:notation>
    <skos:altLabel>water_column_skin</skos:altLabel>
    <dc:date>2006-11-15 08:15:00.0</dc:date>
    <skos:note xml:lang="en">accepted</skos:note>
    <skos:altLabel xml:lang="en">water_column_skin</skos:altLabel>
    <skos:prefLabel xml:lang="en">water column skin</skos:prefLabel>
    <rdf:type rdf:resource="http://www.w3.org/2004/02/skos/core#Concept" />
    <void:inDataset rdf:resource="http://vocab.nerc.ac.uk/.well-known/void" />
    <dc:identifier>SDN:L13::WS</dc:identifier>
  </rdf:Description>
  <rdf:Description rdf:about="http://vocab.nerc.ac.uk/collection/L13/current/AB/">
    <skos:inScheme rdf:resource="http://vocab.nerc.ac.uk/scheme/NETOC_VCOV/current/" />
    <skos:related rdf:resource="http://vocab.nerc.ac.uk/collection/P25/current/WINDT/" />
    <skos:altLabel>atmosphere_boundary</skos:altLabel>
    <skos:altLabel xml:lang="en">atmosphere_boundary</skos:altLabel>
    <skos:definition xml:lang="en">The region of the atmosphere close enough to the Earth's surface for frictional effects of that surface to be significant. Typically not more than 1 km thick.</skos:definition>
    <skos:notation>SDN:L13::AB</skos:notation>
    <pav:version>1</pav:version>
    <skos:note xml:lang="en">accepted</skos:note>
    <skos:related rdf:resource="http://vocab.nerc.ac.uk/collection/P25/current/WINDS/" />
    <skos:related rdf:resource="http://vocab.nerc.ac.uk/collection/P25/current/WINDF/" />
    <dc:date>2006-11-15 08:15:00.0</dc:date>
    <rdf:type rdf:resource="http://www.w3.org/2004/02/skos/core#Concept" />
    <skos:prefLabel xml:lang="en">atmospheric boundary layer</skos:prefLabel>
    <skos:related rdf:resource="http://vocab.nerc.ac.uk/collection/P25/current/ATEMP/" />
    <dc:identifier>SDN:L13::AB</dc:identifier>
    <skos:related rdf:resource="http://vocab.nerc.ac.uk/collection/P25/current/SNWLR/" />
    <pav:hasCurrentVersion rdf:resource="http://vocab.nerc.ac.uk/collection/L13/current/AB/1/" />
    <owl:versionInfo>1</owl:versionInfo>
    <skos:broader rdf:resource="http://vocab.nerc.ac.uk/collection/L19/current/SDNKG16/" />
    <skos:inScheme rdf:resource="http://vocab.nerc.ac.uk/scheme/NETMAR_OCEAN/current/" />
    <void:inDataset rdf:resource="http://vocab.nerc.ac.uk/.well-known/void" />
    <pav:authoredOn>2006-11-15 08:15:00.0</pav:authoredOn>
    <dce:identifier>SDN:L13::AB</dce:identifier>
    <skos:related rdf:resource="http://vocab.nerc.ac.uk/collection/P25/current/WINDY/" />
    <skos:related rdf:resource="http://vocab.nerc.ac.uk/collection/P25/current/WINDX/" />
    <owl:deprecated>false</owl:deprecated>
  </rdf:Description>
  <rdf:Description rdf:about="http://vocab.nerc.ac.uk/collection/L13/current/IA/">
    <dc:identifier>SDN:L13::IA</dc:identifier>
    <void:inDataset rdf:resource="http://vocab.nerc.ac.uk/.well-known/void" />
    <owl:versionInfo>1</owl:versionInfo>
    <pav:version>1</pav:version>
    <skos:prefLabel xml:lang="en">inapplicable</skos:prefLabel>
    <owl:deprecated>false</owl:deprecated>
    <skos:broader rdf:resource="http://vocab.nerc.ac.uk/collection/L19/current/SDNKG16/" />
    <dce:identifier>SDN:L13::IA</dce:identifier>
    <skos:definition xml:lang="en">There is no appropriate value</skos:definition>
    <pav:hasCurrentVersion rdf:resource="http://vocab.nerc.ac.uk/collection/L13/current/IA/1/" />
    <rdf:type rdf:resource="http://www.w3.org/2004/02/skos/core#Concept" />
    <skos:note xml:lang="en">accepted</skos:note>
    <skos:altLabel>inapplicable</skos:altLabel>
    <skos:notation>SDN:L13::IA</skos:notation>
    <pav:authoredOn>2010-02-26 14:44:55.0</pav:authoredOn>
    <dc:date>2010-02-26 14:44:55.0</dc:date>
  </rdf:Description>
  <rdf:Description rdf:about="http://vocab.nerc.ac.uk/collection/L13/current/">
    <skos:member rdf:resource="http://vocab.nerc.ac.uk/collection/L13/current/HP/" />
    <owl:versionInfo>5</owl:versionInfo>
    <rdfs:comment>Group set up under the joint auspices of the SeaDataNet project and the Intergovernmental Oceanographic Commission MarineXML Steering Group for controlled vocabulary governance in the marine domain</rdfs:comment>
    <skos:member rdf:resource="http://vocab.nerc.ac.uk/collection/L13/current/IA/" />
    <dc:title>SeaVoX Vertical Co-ordinate Coverages</dc:title>
    <skos:member rdf:resource="http://vocab.nerc.ac.uk/collection/L13/current/SB/" />
    <skos:member rdf:resource="http://vocab.nerc.ac.uk/collection/L13/current/MA/" />
    <dc:date>2020-05-21 03:00:01.0</dc:date>
    <skos:member rdf:resource="http://vocab.nerc.ac.uk/collection/L13/current/CR/" />
    <dc:publisher>Natural Environment Research Council</dc:publisher>
    <skos:member rdf:resource="http://vocab.nerc.ac.uk/collection/L13/current/BB/" />
    <skos:member rdf:resource="http://vocab.nerc.ac.uk/collection/L13/current/MW/" />
    <skos:member rdf:resource="http://vocab.nerc.ac.uk/collection/L13/current/LI/" />
    <skos:member rdf:resource="http://vocab.nerc.ac.uk/collection/L13/current/TH/" />
    <skos:member rdf:resource="http://vocab.nerc.ac.uk/collection/L13/current/DC/" />
    <dc:description>Terms used to describe data coverage over the vertical (z) co-ordinate.</dc:description>
    <skos:member rdf:resource="http://vocab.nerc.ac.uk/collection/L13/current/MP/" />
    <grg:RE_RegisterOwner>SeaDataNet and MarineXML Vocabulary Content Governance Group</grg:RE_RegisterOwner>
    <skos:member rdf:resource="http://vocab.nerc.ac.uk/collection/L13/current/HX/" />
    <grg:RE_RegisterManager>British Oceanographic Data Centre</grg:RE_RegisterManager>
    <skos:member rdf:resource="http://vocab.nerc.ac.uk/collection/L13/current/AB/" />
    <dc:license rdf:resource="https://creativecommons.org/licenses/by/4.0/" />
    <skos:member rdf:resource="http://vocab.nerc.ac.uk/collection/L13/current/U2/" />
    <skos:member rdf:resource="http://vocab.nerc.ac.uk/collection/L13/current/BP/" />
    <skos:member rdf:resource="http://vocab.nerc.ac.uk/collection/L13/current/MS/" />
    <skos:member rdf:resource="http://vocab.nerc.ac.uk/collection/L13/current/AT/" />
    <skos:member rdf:resource="http://vocab.nerc.ac.uk/collection/L13/current/SP/" />
    <skos:member rdf:resource="http://vocab.nerc.ac.uk/collection/L13/current/ES/" />
    <skos:member rdf:resource="http://vocab.nerc.ac.uk/collection/L13/current/TS/" />
    <skos:member rdf:resource="http://vocab.nerc.ac.uk/collection/L13/current/NS/" />
    <skos:member rdf:resource="http://vocab.nerc.ac.uk/collection/L13/current/TZ/" />
    <skos:prefLabel>SeaVoX Vertical Co-ordinate Coverages</skos:prefLabel>
    <dc:alternative>SeaVoX Vertical Coverages</dc:alternative>
    <skos:member rdf:resource="http://vocab.nerc.ac.uk/collection/L13/current/CO/" />
    <skos:member rdf:resource="http://vocab.nerc.ac.uk/collection/L13/current/SS/" />
    <skos:member rdf:resource="http://vocab.nerc.ac.uk/collection/L13/current/UK/" />
    <skos:member rdf:resource="http://vocab.nerc.ac.uk/collection/L13/current/NB/" />
    <skos:member rdf:resource="http://vocab.nerc.ac.uk/collection/L13/current/WC/" />
    <skos:member rdf:resource="http://vocab.nerc.ac.uk/collection/L13/current/IL/" />
    <skos:member rdf:resource="http://vocab.nerc.ac.uk/collection/L13/current/AP/" />
    <skos:member rdf:resource="http://vocab.nerc.ac.uk/collection/L13/current/SD/" />
    <skos:member rdf:resource="http://vocab.nerc.ac.uk/collection/L13/current/WS/" />
    <skos:altLabel>SeaVoX Vertical Coverages</skos:altLabel>
    <rdf:type rdf:resource="http://www.w3.org/2004/02/skos/core#Collection" />
    <skos:member rdf:resource="http://vocab.nerc.ac.uk/collection/L13/current/HW/" />
    <skos:member rdf:resource="http://vocab.nerc.ac.uk/collection/L13/current/HS/" />
    <skos:member rdf:resource="http://vocab.nerc.ac.uk/collection/L13/current/US/" />
    <skos:member rdf:resource="http://vocab.nerc.ac.uk/collection/L13/current/AY/" />
    <skos:member rdf:resource="http://vocab.nerc.ac.uk/collection/L13/current/CL/" />
    <dc:creator>SeaDataNet and MarineXML Vocabulary Content Governance Group</dc:creator>
    <skos:member rdf:resource="http://vocab.nerc.ac.uk/collection/L13/current/TP/" />
    <skos:member rdf:resource="http://vocab.nerc.ac.uk/collection/L13/current/U1/" />
  </rdf:Description>
  <rdf:Description rdf:about="http://vocab.nerc.ac.uk/collection/L13/current/UK/">
    <skos:definition xml:lang="en">The correct value is not known to, and not computable by, the sender of this data. However, a correct value probably exists.</skos:definition>
    <pav:authoredOn>2006-11-15 08:15:00.0</pav:authoredOn>
    <skos:altLabel>unknown</skos:altLabel>
    <skos:prefLabel xml:lang="en">unknown</skos:prefLabel>
    <pav:hasCurrentVersion rdf:resource="http://vocab.nerc.ac.uk/collection/L13/current/UK/1/" />
    <skos:note xml:lang="en">accepted</skos:note>
    <dc:date>2006-11-15 08:15:00.0</dc:date>
    <void:inDataset rdf:resource="http://vocab.nerc.ac.uk/.well-known/void" />
    <owl:versionInfo>1</owl:versionInfo>
    <rdf:type rdf:resource="http://www.w3.org/2004/02/skos/core#Concept" />
    <skos:notation>SDN:L13::UK</skos:notation>
    <owl:deprecated>false</owl:deprecated>
    <pav:version>1</pav:version>
    <dc:identifier>SDN:L13::UK</dc:identifier>
    <dce:identifier>SDN:L13::UK</dce:identifier>
    <skos:broader rdf:resource="http://vocab.nerc.ac.uk/collection/L19/current/SDNKG16/" />
  </rdf:Description>
  <rdf:Description rdf:about="http://vocab.nerc.ac.uk/collection/L13/current/SD/">
    <owl:deprecated>false</owl:deprecated>
    <skos:definition xml:lang="en">The unlithified sediments (of any grain size from silt to boulders) that form a layer between the solid crust and either the atmosphere or the water column.</skos:definition>
    <dc:identifier>SDN:L13::SD</dc:identifier>
    <pav:hasVersion rdf:resource="http://vocab.nerc.ac.uk/collection/L13/current/SD/1/" />
    <skos:note xml:lang="en">accepted</skos:note>
    <pav:hasCurrentVersion rdf:resource="http://vocab.nerc.ac.uk/collection/L13/current/SD/2/" />
    <owl:versionInfo>2</owl:versionInfo>
    <pav:version>2</pav:version>
    <void:inDataset rdf:resource="http://vocab.nerc.ac.uk/.well-known/void" />
    <skos:broader rdf:resource="http://vocab.nerc.ac.uk/collection/L19/current/SDNKG16/" />
    <skos:notation>SDN:L13::SD</skos:notation>
    <skos:altLabel>sediment</skos:altLabel>
    <skos:prefLabel xml:lang="en">soil and sediment</skos:prefLabel>
    <pav:authoredOn>2010-05-17 15:26:07.0</pav:authoredOn>
    <dc:date>2010-05-17 15:26:07.0</dc:date>
    <rdf:type rdf:resource="http://www.w3.org/2004/02/skos/core#Concept" />
    <dce:identifier>SDN:L13::SD</dce:identifier>
  </rdf:Description>
  <rdf:Description rdf:about="http://vocab.nerc.ac.uk/collection/L13/current/HW/">
    <dc:date>2006-11-15 08:15:00.0</dc:date>
    <skos:notation>SDN:L13::HW</skos:notation>
    <owl:versionInfo>1</owl:versionInfo>
    <skos:broader rdf:resource="http://vocab.nerc.ac.uk/collection/L19/current/SDNKG16/" />
    <skos:related rdf:resource="http://vocab.nerc.ac.uk/collection/P25/current/PO4/" />
    <skos:related rdf:resource="http://vocab.nerc.ac.uk/collection/P25/current/NO3NO2/" />
    <skos:note xml:lang="en">accepted</skos:note>
    <skos:related rdf:resource="http://vocab.nerc.ac.uk/collection/P25/current/NO3/" />
    <skos:related rdf:resource="http://vocab.nerc.ac.uk/collection/P25/current/WTEMP/" />
    <skos:related rdf:resource="http://vocab.nerc.ac.uk/collection/P25/current/SLCA/" />
    <rdf:type rdf:resource="http://www.w3.org/2004/02/skos/core#Concept" />
    <skos:related rdf:resource="http://vocab.nerc.ac.uk/collection/P25/current/SALIN/" />
    <skos:altLabel>hadopelagic</skos:altLabel>
    <pav:authoredOn>2006-11-15 08:15:00.0</pav:authoredOn>
    <pav:version>1</pav:version>
    <dce:identifier>SDN:L13::HW</dce:identifier>
    <skos:related rdf:resource="http://vocab.nerc.ac.uk/collection/P25/current/NO2/" />
    <dc:identifier>SDN:L13::HW</dc:identifier>
    <skos:definition xml:lang="en">The zone of the water column occupying ocean trenches, deeper than approximately 6000 metres.</skos:definition>
    <void:inDataset rdf:resource="http://vocab.nerc.ac.uk/.well-known/void" />
    <pav:hasCurrentVersion rdf:resource="http://vocab.nerc.ac.uk/collection/L13/current/HW/1/" />
    <owl:deprecated>false</owl:deprecated>
    <skos:prefLabel xml:lang="en">hadopelagic water column</skos:prefLabel>
  </rdf:Description>
  <rdf:Description rdf:about="http://vocab.nerc.ac.uk/collection/L13/current/HX/">
    <owl:deprecated>false</owl:deprecated>
    <pav:version>1</pav:version>
    <void:inDataset rdf:resource="http://vocab.nerc.ac.uk/.well-known/void" />
    <skos:related rdf:resource="http://vocab.nerc.ac.uk/collection/P25/current/ATEMP/" />
    <owl:versionInfo>1</owl:versionInfo>
    <dce:identifier>SDN:L13::HX</dce:identifier>
    <skos:note xml:lang="en">accepted</skos:note>
    <skos:definition xml:lang="en">The region of the atmosphere where the mixing ratio of gases is differentiated by gravity. Lies above the homosphere, from about 100 km in altitude.</skos:definition>
    <skos:altLabel>heterosphere</skos:altLabel>
    <dc:identifier>SDN:L13::HX</dc:identifier>
    <pav:authoredOn>2006-11-15 08:15:00.0</pav:authoredOn>
    <skos:broader rdf:resource="http://vocab.nerc.ac.uk/collection/L19/current/SDNKG16/" />
    <skos:notation>SDN:L13::HX</skos:notation>
    <dc:date>2006-11-15 08:15:00.0</dc:date>
    <skos:prefLabel xml:lang="en">heterosphere</skos:prefLabel>
    <pav:hasCurrentVersion rdf:resource="http://vocab.nerc.ac.uk/collection/L13/current/HX/1/" />
    <rdf:type rdf:resource="http://www.w3.org/2004/02/skos/core#Concept" />
  </rdf:Description>
  <rdf:Description rdf:about="http://vocab.nerc.ac.uk/collection/L13/current/MA/">
    <void:inDataset rdf:resource="http://vocab.nerc.ac.uk/.well-known/void" />
    <owl:versionInfo>1</owl:versionInfo>
    <skos:definition xml:lang="en">The layer of basic (i.e ferromagnesian) solid rock between the core and the crust.  Typically from between 5-70 km below the surface to approximately 2900 km below the surface.</skos:definition>
    <dce:identifier>SDN:L13::MA</dce:identifier>
    <skos:note xml:lang="en">accepted</skos:note>
    <dc:date>2006-11-15 08:15:00.0</dc:date>
    <dc:identifier>SDN:L13::MA</dc:identifier>
    <skos:altLabel>mantle</skos:altLabel>
    <pav:version>1</pav:version>
    <skos:prefLabel xml:lang="en">mantle</skos:prefLabel>
    <pav:authoredOn>2006-11-15 08:15:00.0</pav:authoredOn>
    <owl:deprecated>false</owl:deprecated>
    <pav:hasCurrentVersion rdf:resource="http://vocab.nerc.ac.uk/collection/L13/current/MA/1/" />
    <skos:broader rdf:resource="http://vocab.nerc.ac.uk/collection/L19/current/SDNKG16/" />
    <rdf:type rdf:resource="http://www.w3.org/2004/02/skos/core#Concept" />
    <skos:notation>SDN:L13::MA</skos:notation>
  </rdf:Description>
  <rdf:Description rdf:about="http://vocab.nerc.ac.uk/collection/L13/current/SB/">
    <skos:broader rdf:resource="http://vocab.nerc.ac.uk/collection/L19/current/SDNKG16/" />
    <skos:altLabel>sediment_boundary</skos:altLabel>
    <skos:prefLabel xml:lang="en">soil and sediment boundary layer</skos:prefLabel>
    <pav:authoredOn>2010-05-17 15:28:38.0</pav:authoredOn>
    <owl:versionInfo>1</owl:versionInfo>
    <pav:version>1</pav:version>
    <owl:deprecated>false</owl:deprecated>
    <void:inDataset rdf:resource="http://vocab.nerc.ac.uk/.well-known/void" />
    <skos:note xml:lang="en">accepted</skos:note>
    <skos:definition xml:lang="en">The upper surface (interface plus surficial substrate) of the layer of unlithified sediments (of any grain size from silt to boulders) that form a layer between the solid crust and either the atmosphere or the water column.</skos:definition>
    <pav:hasCurrentVersion rdf:resource="http://vocab.nerc.ac.uk/collection/L13/current/SB/1/" />
    <dc:date>2010-05-17 15:28:38.0</dc:date>
    <dce:identifier>SDN:L13::SB</dce:identifier>
    <skos:notation>SDN:L13::SB</skos:notation>
    <rdf:type rdf:resource="http://www.w3.org/2004/02/skos/core#Concept" />
    <dc:identifier>SDN:L13::SB</dc:identifier>
  </rdf:Description>
  <rdf:Description rdf:about="http://vocab.nerc.ac.uk/collection/L13/current/WC/">
    <rdf:type rdf:resource="http://www.w3.org/2004/02/skos/core#Concept" />
    <dce:identifier>SDN:L13::WC</dce:identifier>
    <skos:related rdf:resource="http://vocab.nerc.ac.uk/collection/P25/current/NO2/" />
    <owl:deprecated>false</owl:deprecated>
    <void:inDataset rdf:resource="http://vocab.nerc.ac.uk/.well-known/void" />
    <skos:related rdf:resource="http://vocab.nerc.ac.uk/collection/P25/current/TURB/" />
    <skos:note xml:lang="en">accepted</skos:note>
    <skos:related rdf:resource="http://vocab.nerc.ac.uk/collection/P25/current/PHAEO/" />
    <skos:related rdf:resource="http://vocab.nerc.ac.uk/collection/P25/current/OXYS/" />
    <skos:related rdf:resource="http://vocab.nerc.ac.uk/collection/P25/current/SLCA/" />
    <skos:related rdf:resource="http://vocab.nerc.ac.uk/collection/P25/current/PO4/" />
    <pav:hasCurrentVersion rdf:resource="http://vocab.nerc.ac.uk/collection/L13/current/WC/1/" />
    <dc:date>2006-11-15 08:15:00.0</dc:date>
    <pav:version>1</pav:version>
    <owl:versionInfo>1</owl:versionInfo>
    <dc:identifier>SDN:L13::WC</dc:identifier>
    <skos:related rdf:resource="http://vocab.nerc.ac.uk/collection/P25/current/SALIN/" />
    <skos:prefLabel xml:lang="en">water column</skos:prefLabel>
    <pav:authoredOn>2006-11-15 08:15:00.0</pav:authoredOn>
    <skos:inScheme rdf:resource="http://vocab.nerc.ac.uk/scheme/NETMAR_OCEAN/current/" />
    <skos:related rdf:resource="http://vocab.nerc.ac.uk/collection/P25/current/CHLA/" />
    <skos:related rdf:resource="http://vocab.nerc.ac.uk/collection/P25/current/PHYTABUND/" />
    <skos:altLabel>water_column</skos:altLabel>
    <skos:altLabel xml:lang="en">water_column</skos:altLabel>
    <skos:related rdf:resource="http://vocab.nerc.ac.uk/collection/P25/current/NO3NO2/" />
    <skos:inScheme rdf:resource="http://vocab.nerc.ac.uk/scheme/NETOC_VCOV/current/" />
    <skos:related rdf:resource="http://vocab.nerc.ac.uk/collection/P25/current/NO3/" />
    <skos:definition xml:lang="en">The entire body of water between the bed and the atmosphere.</skos:definition>
    <skos:related rdf:resource="http://vocab.nerc.ac.uk/collection/P25/current/DOXY/" />
    <skos:broader rdf:resource="http://vocab.nerc.ac.uk/collection/L19/current/SDNKG16/" />
    <skos:related rdf:resource="http://vocab.nerc.ac.uk/collection/P25/current/WTEMP/" />
    <skos:notation>SDN:L13::WC</skos:notation>
  </rdf:Description>
  <rdf:Description rdf:about="http://vocab.nerc.ac.uk/collection/L13/current/HP/">
    <skos:definition xml:lang="en">The boundary region between the homosphere and the heterosphere. Typically at about 100 km.</skos:definition>
    <dce:identifier>SDN:L13::HP</dce:identifier>
    <pav:authoredOn>2006-11-15 08:15:00.0</pav:authoredOn>
    <skos:broader rdf:resource="http://vocab.nerc.ac.uk/collection/L19/current/SDNKG16/" />
    <skos:notation>SDN:L13::HP</skos:notation>
    <pav:version>1</pav:version>
    <skos:note xml:lang="en">accepted</skos:note>
    <skos:related rdf:resource="http://vocab.nerc.ac.uk/collection/P25/current/ATEMP/" />
    <pav:hasCurrentVersion rdf:resource="http://vocab.nerc.ac.uk/collection/L13/current/HP/1/" />
    <dc:identifier>SDN:L13::HP</dc:identifier>
    <dc:date>2006-11-15 08:15:00.0</dc:date>
    <owl:versionInfo>1</owl:versionInfo>
    <skos:altLabel>homopause</skos:altLabel>
    <owl:deprecated>false</owl:deprecated>
    <rdf:type rdf:resource="http://www.w3.org/2004/02/skos/core#Concept" />
    <void:inDataset rdf:resource="http://vocab.nerc.ac.uk/.well-known/void" />
    <skos:prefLabel xml:lang="en">homopause</skos:prefLabel>
  </rdf:Description>
  <rdf:Description rdf:about="http://vocab.nerc.ac.uk/collection/L13/current/NS/">
    <skos:related rdf:resource="http://vocab.nerc.ac.uk/collection/P25/current/PO4/" />
    <skos:altLabel>water_column_boundary</skos:altLabel>
    <skos:related rdf:resource="http://vocab.nerc.ac.uk/collection/P25/current/ICECOV/" />
    <owl:versionInfo>1</owl:versionInfo>
    <skos:related rdf:resource="http://vocab.nerc.ac.uk/collection/P25/current/ICETYPE/" />
    <pav:version>1</pav:version>
    <skos:related rdf:resource="http://vocab.nerc.ac.uk/collection/P25/current/NO3NO2/" />
    <skos:related rdf:resource="http://vocab.nerc.ac.uk/collection/P25/current/SLCA/" />
    <skos:related rdf:resource="http://vocab.nerc.ac.uk/collection/P25/current/NO2/" />
    <skos:note xml:lang="en">accepted</skos:note>
    <skos:related rdf:resource="http://vocab.nerc.ac.uk/collection/P25/current/SALIN/" />
    <dce:identifier>SDN:L13::NS</dce:identifier>
    <skos:related rdf:resource="http://vocab.nerc.ac.uk/collection/P25/current/PHAEO/" />
    <skos:related rdf:resource="http://vocab.nerc.ac.uk/collection/P25/current/ICETHICK/" />
    <skos:definition xml:lang="en">The zone of the water column that is significantly influenced by the atmosphere. Typically the top 10m of the water column.</skos:definition>
    <skos:prefLabel xml:lang="en">water column boundary layer</skos:prefLabel>
    <skos:related rdf:resource="http://vocab.nerc.ac.uk/collection/P25/current/ICEDIR/" />
    <pav:hasCurrentVersion rdf:resource="http://vocab.nerc.ac.uk/collection/L13/current/NS/1/" />
    <skos:notation>SDN:L13::NS</skos:notation>
    <dc:identifier>SDN:L13::NS</dc:identifier>
    <skos:related rdf:resource="http://vocab.nerc.ac.uk/collection/P25/current/WTEMP/" />
    <skos:related rdf:resource="http://vocab.nerc.ac.uk/collection/P25/current/ICESSALIN/" />
    <void:inDataset rdf:resource="http://vocab.nerc.ac.uk/.well-known/void" />
    <skos:related rdf:resource="http://vocab.nerc.ac.uk/collection/P25/current/ICEEDGE/" />
    <rdf:type rdf:resource="http://www.w3.org/2004/02/skos/core#Concept" />
    <skos:related rdf:resource="http://vocab.nerc.ac.uk/collection/P25/current/ICEBERG/" />
    <skos:related rdf:resource="http://vocab.nerc.ac.uk/collection/P25/current/CHLA/" />
    <skos:related rdf:resource="http://vocab.nerc.ac.uk/collection/P25/current/ICEDISP/" />
    <skos:related rdf:resource="http://vocab.nerc.ac.uk/collection/P25/current/ICESPD/" />
    <skos:broader rdf:resource="http://vocab.nerc.ac.uk/collection/L19/current/SDNKG16/" />
    <dc:date>2006-11-15 08:15:00.0</dc:date>
    <owl:deprecated>false</owl:deprecated>
    <skos:related rdf:resource="http://vocab.nerc.ac.uk/collection/P25/current/ICETEMP/" />
    <skos:related rdf:resource="http://vocab.nerc.ac.uk/collection/P25/current/PHYTABUND/" />
    <skos:related rdf:resource="http://vocab.nerc.ac.uk/collection/P25/current/NO3/" />
    <pav:authoredOn>2006-11-15 08:15:00.0</pav:authoredOn>
  </rdf:Description>
  <rdf:Description rdf:about="http://vocab.nerc.ac.uk/collection/L13/current/HS/">
    <rdf:type rdf:resource="http://www.w3.org/2004/02/skos/core#Concept" />
    <void:inDataset rdf:resource="http://vocab.nerc.ac.uk/.well-known/void" />
    <skos:note xml:lang="en">accepted</skos:note>
    <dce:identifier>SDN:L13::HS</dce:identifier>
    <pav:version>1</pav:version>
    <dc:date>2006-11-15 08:15:00.0</dc:date>
    <owl:versionInfo>1</owl:versionInfo>
    <skos:notation>SDN:L13::HS</skos:notation>
    <pav:hasCurrentVersion rdf:resource="http://vocab.nerc.ac.uk/collection/L13/current/HS/1/" />
    <skos:related rdf:resource="http://vocab.nerc.ac.uk/collection/P25/current/ATEMP/" />
    <dc:identifier>SDN:L13::HS</dc:identifier>
    <owl:deprecated>false</owl:deprecated>
    <skos:altLabel>homosphere</skos:altLabel>
    <skos:prefLabel xml:lang="en">homosphere</skos:prefLabel>
    <skos:definition xml:lang="en">The region of the atmosphere where gases are fully mixed by diffusion and turbulence. Lies between the surface (0 km) and the base of the heterosphere (at about 100 km).</skos:definition>
    <pav:authoredOn>2006-11-15 08:15:00.0</pav:authoredOn>
    <skos:broader rdf:resource="http://vocab.nerc.ac.uk/collection/L19/current/SDNKG16/" />
  </rdf:Description>
  <rdf:Description rdf:about="http://vocab.nerc.ac.uk/collection/L13/current/TZ/">
    <owl:deprecated>false</owl:deprecated>
    <dc:date>2006-11-15 08:15:00.0</dc:date>
    <dc:identifier>SDN:L13::TZ</dc:identifier>
    <pav:hasCurrentVersion rdf:resource="http://vocab.nerc.ac.uk/collection/L13/current/TZ/1/" />
    <skos:notation>SDN:L13::TZ</skos:notation>
    <pav:authoredOn>2006-11-15 08:15:00.0</pav:authoredOn>
    <owl:versionInfo>1</owl:versionInfo>
    <skos:prefLabel xml:lang="en">thermopause</skos:prefLabel>
    <void:inDataset rdf:resource="http://vocab.nerc.ac.uk/.well-known/void" />
    <rdf:type rdf:resource="http://www.w3.org/2004/02/skos/core#Concept" />
    <skos:broader rdf:resource="http://vocab.nerc.ac.uk/collection/L19/current/SDNKG16/" />
    <skos:note xml:lang="en">accepted</skos:note>
    <pav:version>1</pav:version>
    <skos:related rdf:resource="http://vocab.nerc.ac.uk/collection/P25/current/ATEMP/" />
    <dce:identifier>SDN:L13::TZ</dce:identifier>
    <skos:altLabel>thermopause</skos:altLabel>
    <skos:definition xml:lang="en">The boundary between the thermosphere and the exosphere. Typically at about 400 km.</skos:definition>
  </rdf:Description>
  <rdf:Description rdf:about="http://vocab.nerc.ac.uk/collection/L13/current/BP/">
    <dc:identifier>SDN:L13::BP</dc:identifier>
    <skos:related rdf:resource="http://vocab.nerc.ac.uk/collection/P25/current/SALIN/" />
    <skos:related rdf:resource="http://vocab.nerc.ac.uk/collection/P25/current/WTEMP/" />
    <skos:prefLabel xml:lang="en">bathypelagic water column</skos:prefLabel>
    <skos:notation>SDN:L13::BP</skos:notation>
    <owl:deprecated>false</owl:deprecated>
    <skos:broader rdf:resource="http://vocab.nerc.ac.uk/collection/L19/current/SDNKG16/" />
    <dc:date>2006-11-15 08:15:00.0</dc:date>
    <owl:versionInfo>1</owl:versionInfo>
    <skos:related rdf:resource="http://vocab.nerc.ac.uk/collection/P25/current/NO3/" />
    <pav:version>1</pav:version>
    <dce:identifier>SDN:L13::BP</dce:identifier>
    <skos:related rdf:resource="http://vocab.nerc.ac.uk/collection/P25/current/NO2/" />
    <rdf:type rdf:resource="http://www.w3.org/2004/02/skos/core#Concept" />
    <skos:note xml:lang="en">accepted</skos:note>
    <void:inDataset rdf:resource="http://vocab.nerc.ac.uk/.well-known/void" />
    <skos:related rdf:resource="http://vocab.nerc.ac.uk/collection/P25/current/NO3NO2/" />
    <pav:hasCurrentVersion rdf:resource="http://vocab.nerc.ac.uk/collection/L13/current/BP/1/" />
    <pav:authoredOn>2006-11-15 08:15:00.0</pav:authoredOn>
    <skos:related rdf:resource="http://vocab.nerc.ac.uk/collection/P25/current/SLCA/" />
    <skos:definition xml:lang="en">The water column zone illuminated only by bioluminescent organisms. Typically between depths of approximately 1000 metres and 4000 metres.</skos:definition>
    <skos:altLabel>bathypelagic</skos:altLabel>
    <skos:related rdf:resource="http://vocab.nerc.ac.uk/collection/P25/current/PO4/" />
  </rdf:Description>
</rdf:RDF>

